---
layout: post
category: projects
---

This article will be the first part in a series exploring my recent research. 

![Qwen Heatmaps](images/qwen_combined_heatmaps.png)

Pardon our dust! This article will be live soon.

$$ x^{(\ell+1)} = x^{(\ell)} + f(x^{(\ell)}, \theta^{(\ell)}) $$ 

$$ x^{(L)} = x^{(0)} + \sum_{\ell=0}^{L-1} f(x^{(\ell)}, \theta^{(\ell)}) $$

$$ \mathbf{u} \cdot \mathbf{v} = \|\mathbf{u}\| \|\mathbf{v}\| \cos(\theta) $$

$$ \cos(\theta) = \frac{\mathbf{u} \cdot \mathbf{v}}{\|\mathbf{u}\| \|\mathbf{v}\|} $$

$$ f_{\text{cos}}(x) = \frac{1}{2}(x+1) $$

$$ f_{\text{ang}}(x) = 1 - \frac{1}{\pi}\arccos(x) $$

$$ f_{\text{cubic}}(x) = \frac{1}{4} (x^3 + x + 2) $$

$$ f_{\text{sqrt}}(x) = 1 - \sqrt{\frac{1}{2}(1-x)} $$

$$ f_{\text{exp}}(x) = \frac{e^{x} - e^{-1}}{e^1 - e^{-1}} $$
